Better support for partial method application;
this shows up e.g. in `defer` and `go` statements, and previously
required awkward theorems stating things like "calling method Foo with
one argument `rcvr` yields a `(f : val)` such that `f #arg1 ...`
satisfies the spec of method Foo with receiver `rcvr`".
Now, one can states a normal hoare triple, and if a method is partially
applied, that normal spec will later be applicable.

The trick is that this new `method_call` is essentially an eta-expanded
version of the old one, which means the body won't be unfolded until
more arguments are given.

new/golang/defn/globals.v
@@ -60,10 +60,12 @@ Program Definition func_call := sealed @func_call_def.
 Definition func_call_unseal : func_call = _ := seal_eq _.
 
 Definition method_call_def : val :=
-  λ: "pkg_name" "type_name" "method_name",
-    let: (("varAddrs", "functions"), "typeToMethodSets") := globals.unwrap $ GlobalGet "pkg_name" in
-    let: "methodSet" := globals.unwrap $ alist_lookup "type_name" "typeToMethodSets" in
-    globals.unwrap $ alist_lookup "method_name" "methodSet".
+  λ: "pkg_name" "type_name" "method_name" "receiver",
+    (λ: "firstArg",
+       let: (("varAddrs", "functions"), "typeToMethodSets") := globals.unwrap $ GlobalGet "pkg_name" in
+       let: "methodSet" := globals.unwrap $ alist_lookup "type_name" "typeToMethodSets" in
+       (globals.unwrap $ alist_lookup "method_name" "methodSet") "receiver" "firstArg"
+    ).
 Program Definition method_call := sealed @method_call_def.
 Definition method_call_unseal : method_call = _ := seal_eq _.
 
